theories/Algorithmic/Subtyping/Definitions.v
@@ -6,15 +6,15 @@ Import Syntax_Notations.
 Reserved Notation "Γ ⊢a A ⊆ A'" (in custom judg at level 80, Γ custom exp, A custom exp, A' custom exp).
 Reserved Notation "⊢anf A ⊆ A'" (in custom judg at level 80, A custom nf, A' custom nf).
 
-Definition not_univ_pi (A : nf) : Prop :=
+Definition not_univ_pi_sigma (A : nf) : Prop :=
   match A with
-  | nf_typ _ | nf_pi _ _ => False
+  | nf_typ _ | nf_pi _ _ | nf_sigma _ _ => False
   | _ => True
   end.
 
 Inductive alg_subtyping_nf : nf -> nf -> Prop :=
 | asnf_refl : forall A A',
-    not_univ_pi A ->
+    not_univ_pi_sigma A ->
     A = A' ->
     {{ ⊢anf A ⊆ A' }}
 | asnf_univ : forall i j,
@@ -24,6 +24,10 @@ Inductive alg_subtyping_nf : nf -> nf -> Prop :=
     A = A' ->
     {{ ⊢anf B ⊆ B' }} ->
     {{ ⊢anf Π A B ⊆ Π A' B' }}
+| asnf_sigma : forall A B A' B',
+    A = A' ->
+    {{ ⊢anf B ⊆ B' }} ->
+    {{ ⊢anf Σ A B ⊆ Σ A' B' }}
 where "⊢anf A ⊆ A'" := (alg_subtyping_nf A A') (in custom judg) : type_scope.
 
 Inductive alg_subtyping : ctx -> typ -> typ -> Prop :=
