theories/Extraction/Subtyping.v
@@ -30,6 +30,10 @@ Equations subtyping_nf_impl A B : { {{ ⊢anf A ⊆ B }} } + {~ {{ ⊢anf A ⊆ 
     let*b _ := nf_eq_dec A A' while _ in
     let*b _ := subtyping_nf_impl B B' while _ in
     pureb _
+| n{{{ Σ A B }}}, n{{{ Σ A' B' }}} =>
+    let*b _ := nf_eq_dec A A' while _ in
+    let*b _ := subtyping_nf_impl B B' while _ in
+    pureb _
 (** Pseudo-monadic syntax for the next catch-all branch
     generates some unsolved obligations, so we directly match on
     [nf_eq_dec A B] here. *)
